Improved the stack solutions

sol/RefinedStack.fst
@@ -1,19 +1,21 @@
 module RefinedStack
 
-let stack = list int
+abstract let stack = list int
 
-let is_empty s = Nil? s
+abstract let is_empty (s : stack) : GTot bool = Nil? s
 
-let empty = []
+abstract let empty : s:stack{is_empty s} = []
 
-let push i s = i :: s
+abstract let push (i : int) (s0:stack) : s1:stack{~(is_empty s1)} = i :: s0
+abstract let pop (s0:stack{~(is_empty s0)}) : stack = Cons?.tl s0
+abstract let top (s0:stack{~(is_empty s0)}) : int = Cons?.hd s0
 
-let pop (i::s) = s
+let lemma_push_top (s:stack) (i:int) : Lemma (top (push i s) = i) 
+                                         [SMTPat (top (push i s))] = ()
 
-let top (i::s) = i
+let lemma_push_pop (s:stack) (i:int) : Lemma (pop (push i s) == s) 
+                                         [SMTPat (pop (push i s))] = ()
 
-let lemma_push_top s i = ()
-
-let lemma_push_pop s i = ()
-
-let lemma_top_pop_push s = ()
+let lemma_top_pop_push (s:stack{~(is_empty s)}) :
+                                 Lemma (push (top s) (pop s) == s)
+                                   [SMTPat (push (top s) (pop s))] = ()
